Make `branch_caps` more precise
Only include normalisation of the top byte of capability addresses when
the TBI feature is enabled.

This is used in the characterisation of invoked capabilities, so making
this set more precise strengthens our properties.

CHERI_Instantiation.thy
@@ -1378,6 +1378,271 @@ fun caps_of_regval :: "register_value \<Rightarrow> Capability set" where
   "caps_of_regval (Regval_bitvector_129_dec c) = {c}"
 | "caps_of_regval _ = {}"
 
+locale Morello_Bounds_Address_Calculation =
+  fixes translation_el :: "AccType \<Rightarrow> 2 word"
+    and s1_enabled :: "AccType \<Rightarrow> bool"
+    and tbi_enabled :: "AccType \<Rightarrow> nat \<Rightarrow> bool"
+    and in_host :: "AccType \<Rightarrow> bool"
+  assumes tbi_enabled_cong: "\<And>acctype addr1 addr2. bin_nth (int addr1) 55 = bin_nth (int addr2) 55 \<Longrightarrow> tbi_enabled acctype addr1 \<longleftrightarrow> tbi_enabled acctype addr2"
+begin
+
+definition has_ttbr1 :: "AccType \<Rightarrow> bool" where
+  "has_ttbr1 acctype = (translation_el acctype \<in> {EL0, EL1} \<or> in_host acctype)"
+
+definition bounds_address :: "AccType \<Rightarrow> nat \<Rightarrow> nat" where
+  "bounds_address acctype addr =
+     (if tbi_enabled acctype addr then
+        (if s1_enabled acctype \<and> has_ttbr1 acctype \<and> bin_nth (int addr) 55
+         then addr mod 2 ^ 56 + (255 * 2 ^ 56) \<comment> \<open>sign extension of addr[55..0]\<close>
+         else addr mod 2 ^ 56)                 \<comment> \<open>zero extension of addr[55..0]\<close>
+      else addr)"
+
+definition valid_address :: "AccType \<Rightarrow> nat \<Rightarrow> bool" where
+  "valid_address acctype addr \<equiv>
+     (if s1_enabled acctype \<and> has_ttbr1 acctype \<and> bin_nth (int addr) 55
+      then (if tbi_enabled acctype addr
+            then addr mod 2 ^ 56 \<ge> 15 * 2 ^ 52 \<comment> \<open>addr[55..52] = 0xF\<close>
+            else addr \<ge> 4095 * 2 ^ 52)         \<comment> \<open>addr[63..52] = 0xFFF\<close>
+      else (if tbi_enabled acctype addr
+            then addr mod 2 ^ 56 < 2 ^ 52      \<comment> \<open>addr[55..52] = 0x0\<close>
+            else addr < 2 ^ 52))"              \<comment> \<open>addr[63..52] = 0x000\<close>
+
+lemma bin_nth_eq_mod_div:
+  "bin_nth w n = odd (w mod 2 ^ (Suc n) div 2 ^ n)"
+proof -
+  have "bin_nth w n = odd (w div 2 ^ n)"
+    by (auto simp: bin_nth_eq_mod)
+  also have "\<dots> = odd ((w mod 2 ^ (Suc n) + w div 2 ^ (Suc n) * 2 ^ (Suc n)) div 2 ^ n)"
+    unfolding mod_div_mult_eq
+    ..
+  also have "\<dots> = odd ((w mod 2 ^ (Suc n) + (2 ^ n) * (2 * (w div 2 ^ (Suc n)))) div 2 ^ n)"
+    by (auto simp only: mult_ac power_Suc)
+  also have "\<dots> = odd (w mod 2 ^ (Suc n) div 2 ^ n)"
+    by auto
+  finally show ?thesis
+    .
+qed
+
+lemma bin_nth_int_eq_mod_div:
+  "bin_nth (int w) n = odd (w mod 2 ^ (Suc n) div 2 ^ n)"
+proof -
+  have "even (nat (int w mod 2 ^ (Suc n) div 2 ^ n)) = even (int w mod 2 ^ (Suc n) div 2 ^ n)"
+    by (intro even_nat_iff) (auto simp: pos_imp_zdiv_nonneg_iff)
+  then show ?thesis
+    unfolding bin_nth_eq_mod_div nat_mod_as_int
+    by (auto simp: nat_div_distrib nat_power_eq)
+qed
+
+lemma
+  assumes "addr mod 2 ^ 56 \<ge> 15 * 2 ^ 52"
+    and "(addr + offset) mod 2 ^ 56 = addr mod 2 ^ 56 + offset"
+    and "addr mod 2 ^ 56 + offset < 2 ^ 56"
+  shows "bin_nth (int (addr + offset)) 55"
+  using assms
+  unfolding bin_nth_int_eq_mod_div
+  by (auto dest: even_two_times_div_two)
+
+lemma bounds_address_orig_offset_aux:
+  assumes "valid_address acctype addr"
+    and "offset < 2 ^ 52"
+    and "bounds_address acctype addr + offset < 2 ^ 64"
+  shows "bin_nth (int (addr + offset)) 55 = bin_nth (int addr) 55" (is ?bin_nth)
+    and "(addr + offset) mod 2 ^ 56 = addr mod 2 ^ 56 + offset" (is ?addr_mod)
+    (* and "addr mod 2 ^ 56 + offset < 2 ^ 56" (is ?addr_lt) *)
+proof -
+  have "bin_nth (int addr) 55 = bin_nth (int (addr + offset)) 55
+        \<and> (addr + offset) mod 2 ^ 56 = addr mod 2 ^ 56 + offset"
+  proof (cases "s1_enabled acctype \<and> has_ttbr1 acctype \<and> bin_nth (int addr) 55")
+    case True
+    let ?baddr = "bounds_address acctype addr"
+    have "?baddr = (?baddr mod 2 ^ 56) + (?baddr div 2 ^ 56 * 2 ^ 56)"
+      unfolding mod_div_mult_eq
+      ..
+    also have "\<dots> = addr mod 2 ^ 56 + 255 * 2 ^ 56"
+      using True assms(1,3)
+      by (intro arg_cong2[where f = "(+)"])
+         (auto simp add: bounds_address_def valid_address_def simp flip: mod_add_eq)
+    finally have 1: "addr mod 2 ^ 56 + offset < 2 ^ 56" and 2: "addr mod 2 ^ 56 \<ge> 15 * 2 ^ 52"
+      using True assms(1,3)
+      by (auto simp: bounds_address_def valid_address_def split: if_splits)
+    then have 3: "(addr + offset) mod 2 ^ 56 = addr mod 2 ^ 56 + offset"
+      unfolding mod_add_left_eq[of addr "2 ^ 56" offset, symmetric]
+      by auto
+    moreover have "bin_nth (int (addr + offset)) 55"
+      using 1 2 3
+      unfolding bin_nth_int_eq_mod_div
+      by (auto dest: even_two_times_div_two)
+    ultimately show ?thesis
+      using True
+      by auto
+  next
+    case False
+    then have 1: "addr mod 2 ^ 56 < 2 ^ 52"
+      using \<open>valid_address acctype addr\<close>
+      by (auto simp: valid_address_def split: if_splits)
+    then have 2: "addr mod 2 ^ 56 + offset < 2 ^ 53"
+      using \<open>offset < 2 ^ 52\<close>
+      by auto
+    then have 3: "(addr + offset) mod 2 ^ 56 = addr mod 2 ^ 56 + offset"
+      unfolding mod_add_left_eq[of addr "2 ^ 56" offset, symmetric]
+      by auto
+    moreover have "bin_nth (int addr) 55 = bin_nth (int (addr + offset)) 55"
+      using 1 2 3
+      unfolding bin_nth_int_eq_mod_div
+      by auto
+    ultimately show ?thesis
+      by auto
+  qed
+  then show ?bin_nth and ?addr_mod
+    by auto
+qed
+
+lemma bounds_address_offset:
+  assumes "valid_address acctype addr"
+    and "offset < 2 ^ 52"
+    and "bounds_address acctype addr + offset < 2 ^ 64"
+  shows "bounds_address acctype (addr + offset) = bounds_address acctype addr + offset"
+  using bounds_address_orig_offset_aux[OF assms] tbi_enabled_cong[of addr "addr + offset" acctype]
+  by (auto simp: bounds_address_def)
+
+lemma bounds_address_orig_address_no_overflow:
+  assumes "valid_address acctype addr"
+    and "offset < 2 ^ 52"
+    and "bounds_address acctype addr + offset < 2 ^ 64"
+    and "addr < 2 ^ 64"
+  shows "addr + offset < 2 ^ 64"
+proof -
+  have "addr + offset = addr div 2 ^ 56 * 2 ^ 56 + addr mod 2 ^ 56 + offset"
+    by auto
+  also have "\<dots> \<le> 255 * 2 ^ 56 + addr mod 2 ^ 56 + offset"
+    using assms
+    by (intro add_right_mono) auto
+  also have "\<dots> < 2 ^ 64"
+    using bounds_address_orig_offset_aux[OF assms(1-3)]
+    by auto
+  finally show ?thesis .
+qed
+
+end
+
+fun is_isa_exception :: "exception \<Rightarrow> bool" where
+  "is_isa_exception (Error_ExceptionTaken u) = True"
+| "is_isa_exception _ = False"
+
+locale Morello_Fixed_Address_Translation =
+  Morello_Bounds_Address_Calculation + Wellformed_Traces wellformed_ev is_isa_exception
+  for wellformed_ev :: "register_value event \<Rightarrow> bool" +
+  fixes translate_address :: "nat \<Rightarrow> nat option"
+    and is_translation_event :: "register_value event \<Rightarrow> bool"
+    (* TODO: Let assumptions refer to a trace (and possibly a state) instead of just events,
+       allowing us to make assumptions about register values/fields that might change over time,
+       e.g. PSTATE.EL *)
+    and translation_assms :: "register_value event \<Rightarrow> bool"
+    and UNKNOWN_caps :: "Capability set"
+  assumes translate_correct[simp]:
+      "\<And>vaddress acctype iswrite wasaligned size iswritevalidcap addrdesc.
+          Run (AArch64_FullTranslateWithTag vaddress acctype iswrite wasaligned size iswritevalidcap) t addrdesc \<Longrightarrow>
+          \<not>IsFault addrdesc \<Longrightarrow>
+          \<forall>e \<in> set t. translation_assms e \<Longrightarrow>
+          translate_address (unat vaddress) = Some (unat (FullAddress_address (AddressDescriptor_paddress addrdesc)))"
+    and is_translation_event_correct:
+      "\<And>vaddress acctype iswrite wasaligned size iswritevalidcap addrdesc e.
+          Run (AArch64_FullTranslateWithTag vaddress acctype iswrite wasaligned size iswritevalidcap) t addrdesc \<Longrightarrow>
+          \<forall>e' \<in> set t. translation_assms e' \<Longrightarrow>
+          e \<in> set t \<Longrightarrow> is_mem_event e \<Longrightarrow>
+          is_translation_event e"
+    and no_cap_load_translation_events: "\<And>rk addr sz data. \<not>is_translation_event (E_read_memt rk addr sz data)"
+    \<comment> \<open>TODO: Replace the following with an assumption that the original value of PSTATE.EL before
+        it gets overwritten by @{term AArch64_TakeException} or @{term AArch64_ExceptionReturnToCapability}
+        corresponds to @{term translation_el}.\<close>
+    and translation_el: "\<And>t acctype el. Run (AArch64_AccessUsesEL acctype) t el \<Longrightarrow> \<forall>e \<in> set t. translation_assms e \<Longrightarrow> translation_el acctype = el"
+    and s1_enabled: "\<And>t acctype s1e. Run (AArch64_IsStageOneEnabled acctype) t s1e \<Longrightarrow> \<forall>e \<in> set t. translation_assms e \<Longrightarrow> s1_enabled acctype = s1e"
+    and tbi_enabled: "\<And>t acctype addr top. Run (AddrTop addr (translation_el acctype)) t top \<Longrightarrow> \<forall>e \<in> set t. translation_assms e \<Longrightarrow> tbi_enabled acctype (unat addr) = (top \<noteq> 63)"
+    and in_host: "\<And>t acctype ih. Run (ELIsInHost (translation_el acctype)) t ih \<Longrightarrow> \<forall>e \<in> set t. translation_assms e \<Longrightarrow> in_host acctype = ih"
+    and translate_address_valid: "\<And>vaddr acctype paddr. translate_address vaddr = Some paddr \<Longrightarrow> valid_address acctype vaddr"
+    and translate_bounds_address: "\<And>vaddr acctype. valid_address acctype vaddr \<Longrightarrow> translate_address (bounds_address acctype vaddr) = translate_address vaddr"
+    (* Memory pages are at least 4KB in AArch64 *)
+    and translate_address_paged: "\<And>vaddr vaddr' paddr. translate_address vaddr = Some paddr \<Longrightarrow> vaddr' div 2^12 = vaddr div 2^12 \<Longrightarrow> translate_address vaddr' = Some (2^12 * (paddr div 2^12) + vaddr' mod 2^12)"
+    (*and translate_address_paged: "\<And>vaddr vaddr' acctype paddr paddr'. translate_address vaddr acctype = Some paddr \<Longrightarrow> translate_address vaddr' acctype = Some paddr' \<Longrightarrow> vaddr div 2^12 = vaddr' div 2^12 \<Longrightarrow> paddr div 2^12 = paddr' div 2^12"
+    and translate_address_page_offset: "\<And>vaddr acctype paddr. translate_address vaddr acctype = Some paddr \<Longrightarrow> paddr mod 2^12 = vaddr mod 2^12"*)
+    and AArch64_TakeException_raises_isa_ex:
+      "exp_raises_isa_ex (AArch64_TakeException target_el exception preferred_exception_return vect_offset)"
+begin
+
+lemma translate_address_page_offset:
+  assumes "translate_address vaddr = Some paddr"
+  shows "paddr mod 2^12 = vaddr mod 2^12"
+proof -
+  have *: "2^12 * (paddr div 2^12) + vaddr mod 2^12 = paddr"
+    using assms translate_address_paged[of vaddr paddr vaddr]
+    by auto
+  have "(2^12 * (paddr div 2^12) + vaddr mod 2^12) mod 2^12 = vaddr mod 2^12"
+    by simp
+  then show ?thesis
+    unfolding *
+    .
+qed
+
+lemma translate_address_aligned_iff[simp]:
+  assumes "translate_address vaddr = Some paddr"
+    and "sz dvd 2^12"
+  shows "aligned paddr sz \<longleftrightarrow> aligned vaddr sz"
+proof -
+  have "aligned paddr sz \<longleftrightarrow> aligned (2^12 * (paddr div 2^12) + vaddr mod 2^12) sz"
+    using assms translate_address_paged[OF assms(1), where vaddr' = vaddr]
+    by auto
+  also have "\<dots> \<longleftrightarrow> aligned vaddr sz"
+    using assms(2)
+    by (auto simp: aligned_def dvd_add_right_iff dvd_mod_iff)
+  finally show ?thesis
+    .
+qed
+
+lemma AArch64_FullTranslate_translate_address[simp]:
+  assumes "Run (AArch64_FullTranslate vaddress acctype iswrite wasaligned sz) t addrdesc"
+    and "\<not>IsFault addrdesc" and "\<forall>e \<in> set t. translation_assms e"
+  shows "translate_address (unat vaddress) = Some (unat (FullAddress_address (AddressDescriptor_paddress addrdesc)))"
+  using assms
+  by (auto simp: AArch64_FullTranslate_def IsFault_def elim!: Run_bindE Run_ifE)
+
+lemma AArch64_TranslateAddressWithTag_translate_address[simp]:
+  assumes "Run (AArch64_TranslateAddressWithTag vaddress acctype iswrite wasaligned sz iswritevalidcap) t addrdesc"
+    and "\<not>IsFault addrdesc" and "\<forall>e \<in> set t. translation_assms e"
+  shows "translate_address (unat vaddress) = Some (unat (FullAddress_address (AddressDescriptor_paddress addrdesc)))"
+  using assms
+  by (auto simp: AArch64_TranslateAddressWithTag_def IsFault_def elim!: Run_bindE Run_ifE)
+
+lemma AArch64_TranslateAddress_translate_address[simp]:
+  assumes "Run (AArch64_TranslateAddress vaddress acctype iswrite wasaligned sz) t addrdesc"
+    and "\<not>IsFault addrdesc" and "\<forall>e \<in> set t. translation_assms e"
+  shows "translate_address (unat vaddress) = Some (unat (FullAddress_address (AddressDescriptor_paddress addrdesc)))"
+  using assms
+  by (auto simp: AArch64_TranslateAddress_def IsFault_def elim!: Run_bindE Run_ifE)
+
+lemma AArch64_TranslateAddressForAtomicAccess_translate_address[simp]:
+  assumes "Run (AArch64_TranslateAddressForAtomicAccess vaddress sz) t addrdesc"
+    and "\<not>IsFault addrdesc" and "\<forall>e \<in> set t. translation_assms e"
+  shows "translate_address (unat vaddress) = Some (unat (FullAddress_address (AddressDescriptor_paddress addrdesc)))"
+  using assms
+  by (auto simp: AArch64_TranslateAddressForAtomicAccess_def IsFault_def elim!: Run_bindE Run_ifE Run_letE)
+
+(*sublocale Morello_ISA where translate_address = "\<lambda>addr _. translate_address addr"
+  using no_cap_load_translation_events AArch64_TakeException_raises_isa_ex
+  by unfold_locales auto
+
+sublocale Capability_ISA_Fixed_Translation CC ISA UNKNOWN_caps translation_assms
+  by unfold_locales (auto simp: ISA_def)*)
+
+lemma read_reg_PSTATE_translation_el:
+  assumes "Run (read_reg PSTATE_ref :: ProcState M) t a"
+    and "\<forall>e \<in> set t. translation_assms e"
+    and "acctype \<noteq> AccType_UNPRIV"
+  shows "translation_el acctype = ProcState_EL a"
+  using assms
+  by (intro translation_el[where t = t]) (auto simp: AArch64_AccessUsesEL_def)
+
+end
+
 text \<open>Characterisation of invoked capabilities\<close>
 
 fun instr_invokes_code_cap_from_reg :: "instr_ast \<Rightarrow> int option" where
@@ -1530,24 +1795,6 @@ abbreviation mutable_perms where
 definition normalise_cursor_flags :: "Capability \<Rightarrow> bool \<Rightarrow> Capability" where
   "normalise_cursor_flags c top_bit \<equiv> CapSetFlags c (if top_bit then max_word else 0)"
 
-definition branch_caps :: "Capability \<Rightarrow> Capability set" where
-  "branch_caps c \<equiv>
-     (if CapIsSealed c then
-        {c}
-      else
-        {c, normalise_cursor_flags c (CapGetValue c !! 55), normalise_cursor_flags c False,
-         set_bit c 0 False, normalise_cursor_flags (set_bit c 0 False) (CapGetValue c !! 55),
-         normalise_cursor_flags (set_bit c 0 False) False})"
-
-definition mem_branch_caps :: "Capability \<Rightarrow> Capability set" where
-  "mem_branch_caps c \<equiv>
-     (if CapGetObjectType c = CAP_SEAL_TYPE_RB then {c} \<union> branch_caps (CapUnseal c)
-      else if CapIsSealed c then {c}
-      else branch_caps c \<union> branch_caps (clear_perm mutable_perms c))"
-
-definition mem_data_caps :: "Capability \<Rightarrow> Capability set" where
-  "mem_data_caps c \<equiv> (if CapIsSealed c then {c} else {c, clear_perm mutable_perms c})"
-
 fun instr_of_trace :: "register_value trace \<Rightarrow> instr_ast option" where
   "instr_of_trace (E_write_reg r (Regval_instr_ast instr) # _) =
      (if r = ''__ThisInstrAbstract'' then Some instr else None)"
@@ -1606,15 +1853,6 @@ definition trace_has_cap_load_auth :: "register_value trace \<Rightarrow> bool" 
 
 definition trace_uses_mem_caps :: "(register_value, instr) isa_trace \<Rightarrow> bool" where
   "trace_uses_mem_caps t \<equiv> trace_has_cap_load_auth (trace t)"
-
-definition trace_invokes_direct_mem_sentries :: "register_value trace \<Rightarrow> Capability set" where
-  "trace_invokes_direct_mem_sentries t \<equiv>
-     \<Union>{mem_branch_caps c | c. \<exists>e \<in> set t. \<exists>addr sz.
-         trace_is_indirect_branch t \<and>
-         trace_invokes_indirect_sentries t = {} \<and>
-         trace_has_cap_load_auth t \<and>
-         reads_mem_cap CC e = Some (addr, sz, c) \<and>
-         CapIsTagSet c \<and> is_sentry c}"
 
 definition trace_has_system_reg_access :: "register_value trace \<Rightarrow> bool" where
   "trace_has_system_reg_access t \<equiv>
@@ -1701,10 +1939,6 @@ lemma determ_instr_exp_instr_of_exp_Some_cases:
   by (use assms in \<open>auto simp: determ_instr_exp_def no_reg_writes_to_instr_of_exp
                          elim: write_reg_ThisInstrAbstract_Traces_instr_of_trace_cases\<close>)
 
-fun is_isa_exception :: "exception \<Rightarrow> bool" where
-  "is_isa_exception (Error_ExceptionTaken u) = True"
-| "is_isa_exception _ = False"
-
 definition trace_raises_ex :: "(register_value, instr) isa_trace \<Rightarrow> bool" where
   "trace_raises_ex t \<equiv>
      (case trace_kind t of
@@ -1737,8 +1971,9 @@ fun is_mem_event :: "'regval event \<Rightarrow> bool" where
 | "is_mem_event (E_write_mem _ _ _ _ _) = True"
 | "is_mem_event _ = False"
 
-locale Morello_ISA =
-  Wellformed_Traces wellformed_ev is_isa_exception
+locale Morello_ISA = Morello_Fixed_Address_Translation
+  (*Wellformed_Traces wellformed_ev is_isa_exception +
+  Morello_Bounds_Address_Calculation
   for wellformed_ev :: "register_value event \<Rightarrow> bool" +
   fixes translate_address :: "nat \<Rightarrow> acctype \<Rightarrow> nat option" \<comment> \<open>assuming fixed translation throughout trace; TODO: Move Morello_Fixed_Address_Translation locale up\<close>
     and is_translation_event :: "register_value event \<Rightarrow> bool"
@@ -1748,7 +1983,7 @@ locale Morello_ISA =
         @{term AArch64_TakeException}, guaranteeing that the latter will raise an exception rather
         than failing with a type error.\<close>
     and AArch64_TakeException_raises_isa_ex:
-      "exp_raises_isa_ex (AArch64_TakeException target_el exception preferred_exception_return vect_offset)"
+      "exp_raises_isa_ex (AArch64_TakeException target_el exception preferred_exception_return vect_offset)"*)
 begin
 
 abbreviation "translation_control_regs \<equiv>
@@ -1762,6 +1997,36 @@ abbreviation "translation_control_regs \<equiv>
    ''MPAMVPM4_EL2'', ''MPAMVPM5_EL2'', ''MPAMVPM6_EL2'', ''MPAMVPM7_EL2'',
    ''MPAMHCR_EL2''}"
 
+definition branch_caps :: "Capability \<Rightarrow> Capability set" where
+  "branch_caps c \<equiv>
+     (if CapIsSealed c then
+        {c}
+      else
+        ({c, set_bit c 0 False} \<union>
+         (if tbi_enabled AccType_IFETCH (unat (CapGetValue c)) then
+            {normalise_cursor_flags c (CapGetValue c !! 55), normalise_cursor_flags c False,
+             normalise_cursor_flags (set_bit c 0 False) (CapGetValue c !! 55),
+             normalise_cursor_flags (set_bit c 0 False) False}
+          else {})))"
+
+definition mem_branch_caps :: "Capability \<Rightarrow> Capability set" where
+  "mem_branch_caps c \<equiv>
+     (if CapGetObjectType c = CAP_SEAL_TYPE_RB then {c} \<union> branch_caps (CapUnseal c)
+      else if CapIsSealed c then {c}
+      else branch_caps c \<union> branch_caps (clear_perm mutable_perms c))"
+
+definition mem_data_caps :: "Capability \<Rightarrow> Capability set" where
+  "mem_data_caps c \<equiv> (if CapIsSealed c then {c} else {c, clear_perm mutable_perms c})"
+
+definition trace_invokes_direct_mem_sentries :: "register_value trace \<Rightarrow> Capability set" where
+  "trace_invokes_direct_mem_sentries t \<equiv>
+     \<Union>{mem_branch_caps c | c. \<exists>e \<in> set t. \<exists>addr sz.
+         trace_is_indirect_branch t \<and>
+         trace_invokes_indirect_sentries t = {} \<and>
+         trace_has_cap_load_auth t \<and>
+         reads_mem_cap CC e = Some (addr, sz, c) \<and>
+         CapIsTagSet c \<and> is_sentry c}"
+
 definition trace_indirectly_invokes_code_caps :: "register_value trace \<Rightarrow> Capability set" where
   "trace_indirectly_invokes_code_caps t \<equiv>
      {c. \<exists>rk vaddr paddr sz bytes tag sentry c'.
@@ -1769,7 +2034,7 @@ definition trace_indirectly_invokes_code_caps :: "register_value trace \<Rightar
             sentry \<in> trace_invokes_indirect_sentries t \<and>
             \<comment> \<open>TODO: Do we need this: set (address_range vaddr sz) \<subseteq> get_mem_region CC sentry \<and>\<close>
             (trace_indirect_sentry_type t = Some Points_to_Pair \<longrightarrow> vaddr = unat (CapGetValue sentry + 16)) \<and>
-            translate_address vaddr Load = Some paddr \<and>
+            translate_address vaddr = Some paddr \<and>
             E_read_memt rk paddr sz (bytes, tag) \<in> set t \<and>
             cap_of_mem_bytes bytes tag = Some c' \<and> CapIsTagSet c' \<and>
             c \<in> mem_branch_caps c'}"
@@ -1795,7 +2060,7 @@ definition trace_indirectly_invokes_data_caps :: "register_value trace \<Rightar
           {c. \<exists>rk paddr sz bytes tag sentry c'.
                  sz = nat CAPABILITY_DBYTES \<and>
                  sentry \<in> trace_invokes_indirect_sentries t \<and>
-                 translate_address (unat (CapGetValue sentry)) Load = Some paddr \<and>
+                 translate_address (unat (CapGetValue sentry)) = Some paddr \<and>
                  E_read_memt rk paddr sz (bytes, tag) \<in> set t \<and>
                  cap_of_mem_bytes bytes tag = Some c' \<and> CapIsTagSet c' \<and>
                  c \<in> mem_data_caps c'}
@@ -1843,7 +2108,7 @@ definition "ISA \<equiv>
    read_exception_regs = {''VBAR_EL1'', ''VBAR_EL2'', ''VBAR_EL3''},
    write_exception_regs = {},
    isa.is_translation_event = is_translation_event,
-   isa.translate_address = \<lambda>vaddr acctype _. translate_address vaddr acctype\<rparr>"
+   isa.translate_address = \<lambda>vaddr _ _. translate_address vaddr\<rparr>"
 
 sublocale Capability_Invariant_ISA CC ISA UNKNOWN_caps cap_invariant ..
 
@@ -1868,12 +2133,15 @@ lemma ISA_simps[simp]:
   "\<And>instr t. isa.instr_invokes_indirect_caps ISA instr t = instr_invokes_indirect_caps instr t"
   "isa.indirect_pair_sentry_code_offset ISA = 16"
   "isa.indirect_pair_sentry_data_offset ISA = 0"
-  "\<And>vaddr acctype t. isa.translate_address ISA vaddr acctype t = translate_address vaddr acctype"
+  "\<And>vaddr acctype t. isa.translate_address ISA vaddr acctype t = translate_address vaddr"
   by (auto simp: ISA_def)
 
 lemma address_tag_aligned_iff_aligned_16[simp]:
   "address_tag_aligned ISA addr \<longleftrightarrow> aligned addr 16"
   by (auto simp: address_tag_aligned_def aligned_def)
+
+sublocale Capability_ISA_Fixed_Translation CC ISA UNKNOWN_caps translation_assms
+  by unfold_locales (auto simp: ISA_def)
 
 end
 
@@ -1925,153 +2193,6 @@ next
     by (elim set_regval_Some_type_cases; cases r' rule: get_regval_type_cases) auto
 qed
 
-locale Morello_Bounds_Address_Calculation =
-  fixes translation_el :: "AccType \<Rightarrow> 2 word"
-    and s1_enabled :: "AccType \<Rightarrow> bool"
-    and tbi_enabled :: "AccType \<Rightarrow> nat \<Rightarrow> bool"
-    and in_host :: "AccType \<Rightarrow> bool"
-  assumes tbi_enabled_cong: "\<And>acctype addr1 addr2. bin_nth (int addr1) 55 = bin_nth (int addr2) 55 \<Longrightarrow> tbi_enabled acctype addr1 \<longleftrightarrow> tbi_enabled acctype addr2"
-begin
-
-definition has_ttbr1 :: "AccType \<Rightarrow> bool" where
-  "has_ttbr1 acctype = (translation_el acctype \<in> {EL0, EL1} \<or> in_host acctype)"
-
-definition bounds_address :: "AccType \<Rightarrow> nat \<Rightarrow> nat" where
-  "bounds_address acctype addr =
-     (if tbi_enabled acctype addr then
-        (if s1_enabled acctype \<and> has_ttbr1 acctype \<and> bin_nth (int addr) 55
-         then addr mod 2 ^ 56 + (255 * 2 ^ 56) \<comment> \<open>sign extension of addr[55..0]\<close>
-         else addr mod 2 ^ 56)                 \<comment> \<open>zero extension of addr[55..0]\<close>
-      else addr)"
-
-definition valid_address :: "AccType \<Rightarrow> nat \<Rightarrow> bool" where
-  "valid_address acctype addr \<equiv>
-     (if s1_enabled acctype \<and> has_ttbr1 acctype \<and> bin_nth (int addr) 55
-      then (if tbi_enabled acctype addr
-            then addr mod 2 ^ 56 \<ge> 15 * 2 ^ 52 \<comment> \<open>addr[55..52] = 0xF\<close>
-            else addr \<ge> 4095 * 2 ^ 52)         \<comment> \<open>addr[63..52] = 0xFFF\<close>
-      else (if tbi_enabled acctype addr
-            then addr mod 2 ^ 56 < 2 ^ 52      \<comment> \<open>addr[55..52] = 0x0\<close>
-            else addr < 2 ^ 52))"              \<comment> \<open>addr[63..52] = 0x000\<close>
-
-lemma bin_nth_eq_mod_div:
-  "bin_nth w n = odd (w mod 2 ^ (Suc n) div 2 ^ n)"
-proof -
-  have "bin_nth w n = odd (w div 2 ^ n)"
-    by (auto simp: bin_nth_eq_mod)
-  also have "\<dots> = odd ((w mod 2 ^ (Suc n) + w div 2 ^ (Suc n) * 2 ^ (Suc n)) div 2 ^ n)"
-    unfolding mod_div_mult_eq
-    ..
-  also have "\<dots> = odd ((w mod 2 ^ (Suc n) + (2 ^ n) * (2 * (w div 2 ^ (Suc n)))) div 2 ^ n)"
-    by (auto simp only: mult_ac power_Suc)
-  also have "\<dots> = odd (w mod 2 ^ (Suc n) div 2 ^ n)"
-    by auto
-  finally show ?thesis
-    .
-qed
-
-lemma bin_nth_int_eq_mod_div:
-  "bin_nth (int w) n = odd (w mod 2 ^ (Suc n) div 2 ^ n)"
-proof -
-  have "even (nat (int w mod 2 ^ (Suc n) div 2 ^ n)) = even (int w mod 2 ^ (Suc n) div 2 ^ n)"
-    by (intro even_nat_iff) (auto simp: pos_imp_zdiv_nonneg_iff)
-  then show ?thesis
-    unfolding bin_nth_eq_mod_div nat_mod_as_int
-    by (auto simp: nat_div_distrib nat_power_eq)
-qed
-
-lemma
-  assumes "addr mod 2 ^ 56 \<ge> 15 * 2 ^ 52"
-    and "(addr + offset) mod 2 ^ 56 = addr mod 2 ^ 56 + offset"
-    and "addr mod 2 ^ 56 + offset < 2 ^ 56"
-  shows "bin_nth (int (addr + offset)) 55"
-  using assms
-  unfolding bin_nth_int_eq_mod_div
-  by (auto dest: even_two_times_div_two)
-
-lemma bounds_address_orig_offset_aux:
-  assumes "valid_address acctype addr"
-    and "offset < 2 ^ 52"
-    and "bounds_address acctype addr + offset < 2 ^ 64"
-  shows "bin_nth (int (addr + offset)) 55 = bin_nth (int addr) 55" (is ?bin_nth)
-    and "(addr + offset) mod 2 ^ 56 = addr mod 2 ^ 56 + offset" (is ?addr_mod)
-    (* and "addr mod 2 ^ 56 + offset < 2 ^ 56" (is ?addr_lt) *)
-proof -
-  have "bin_nth (int addr) 55 = bin_nth (int (addr + offset)) 55
-        \<and> (addr + offset) mod 2 ^ 56 = addr mod 2 ^ 56 + offset"
-  proof (cases "s1_enabled acctype \<and> has_ttbr1 acctype \<and> bin_nth (int addr) 55")
-    case True
-    let ?baddr = "bounds_address acctype addr"
-    have "?baddr = (?baddr mod 2 ^ 56) + (?baddr div 2 ^ 56 * 2 ^ 56)"
-      unfolding mod_div_mult_eq
-      ..
-    also have "\<dots> = addr mod 2 ^ 56 + 255 * 2 ^ 56"
-      using True assms(1,3)
-      by (intro arg_cong2[where f = "(+)"])
-         (auto simp add: bounds_address_def valid_address_def simp flip: mod_add_eq)
-    finally have 1: "addr mod 2 ^ 56 + offset < 2 ^ 56" and 2: "addr mod 2 ^ 56 \<ge> 15 * 2 ^ 52"
-      using True assms(1,3)
-      by (auto simp: bounds_address_def valid_address_def split: if_splits)
-    then have 3: "(addr + offset) mod 2 ^ 56 = addr mod 2 ^ 56 + offset"
-      unfolding mod_add_left_eq[of addr "2 ^ 56" offset, symmetric]
-      by auto
-    moreover have "bin_nth (int (addr + offset)) 55"
-      using 1 2 3
-      unfolding bin_nth_int_eq_mod_div
-      by (auto dest: even_two_times_div_two)
-    ultimately show ?thesis
-      using True
-      by auto
-  next
-    case False
-    then have 1: "addr mod 2 ^ 56 < 2 ^ 52"
-      using \<open>valid_address acctype addr\<close>
-      by (auto simp: valid_address_def split: if_splits)
-    then have 2: "addr mod 2 ^ 56 + offset < 2 ^ 53"
-      using \<open>offset < 2 ^ 52\<close>
-      by auto
-    then have 3: "(addr + offset) mod 2 ^ 56 = addr mod 2 ^ 56 + offset"
-      unfolding mod_add_left_eq[of addr "2 ^ 56" offset, symmetric]
-      by auto
-    moreover have "bin_nth (int addr) 55 = bin_nth (int (addr + offset)) 55"
-      using 1 2 3
-      unfolding bin_nth_int_eq_mod_div
-      by auto
-    ultimately show ?thesis
-      by auto
-  qed
-  then show ?bin_nth and ?addr_mod
-    by auto
-qed
-
-lemma bounds_address_offset:
-  assumes "valid_address acctype addr"
-    and "offset < 2 ^ 52"
-    and "bounds_address acctype addr + offset < 2 ^ 64"
-  shows "bounds_address acctype (addr + offset) = bounds_address acctype addr + offset"
-  using bounds_address_orig_offset_aux[OF assms] tbi_enabled_cong[of addr "addr + offset" acctype]
-  by (auto simp: bounds_address_def)
-
-lemma bounds_address_orig_address_no_overflow:
-  assumes "valid_address acctype addr"
-    and "offset < 2 ^ 52"
-    and "bounds_address acctype addr + offset < 2 ^ 64"
-    and "addr < 2 ^ 64"
-  shows "addr + offset < 2 ^ 64"
-proof -
-  have "addr + offset = addr div 2 ^ 56 * 2 ^ 56 + addr mod 2 ^ 56 + offset"
-    by auto
-  also have "\<dots> \<le> 255 * 2 ^ 56 + addr mod 2 ^ 56 + offset"
-    using assms
-    by (intro add_right_mono) auto
-  also have "\<dots> < 2 ^ 64"
-    using bounds_address_orig_offset_aux[OF assms(1-3)]
-    by auto
-  finally show ?thesis .
-qed
-
-end
-
 lemma CapSetFlags_mask_56_normalise_cursor_flags:
   "CapSetFlags c (CapGetValue c AND mask 56) = normalise_cursor_flags c False"
   unfolding CapSetFlags_def normalise_cursor_flags_def
@@ -2085,109 +2206,6 @@ lemma CapSetFlags_SignExtend_normalise_cursor_flags:
   unfolding CapSetFlags_def normalise_cursor_flags_def SignExtend1_def sign_extend_def
   by (intro word_eqI)
      (auto simp: update_subrange_vec_dec_test_bit nth_slice nth_scast nth_ucast)
-
-locale Morello_Fixed_Address_Translation =
-  Morello_Bounds_Address_Calculation + Wellformed_Traces wellformed_ev is_isa_exception
-  for wellformed_ev :: "register_value event \<Rightarrow> bool" +
-  fixes translate_address :: "nat \<Rightarrow> nat option"
-    and is_translation_event :: "register_value event \<Rightarrow> bool"
-    (* TODO: Let assumptions refer to a trace (and possibly a state) instead of just events,
-       allowing us to make assumptions about register values/fields that might change over time,
-       e.g. PSTATE.EL *)
-    and translation_assms :: "register_value event \<Rightarrow> bool"
-    and UNKNOWN_caps :: "Capability set"
-  assumes translate_correct[simp]:
-      "\<And>vaddress acctype iswrite wasaligned size iswritevalidcap addrdesc.
-          Run (AArch64_FullTranslateWithTag vaddress acctype iswrite wasaligned size iswritevalidcap) t addrdesc \<Longrightarrow>
-          \<not>IsFault addrdesc \<Longrightarrow>
-          \<forall>e \<in> set t. translation_assms e \<Longrightarrow>
-          translate_address (unat vaddress) = Some (unat (FullAddress_address (AddressDescriptor_paddress addrdesc)))"
-    and is_translation_event_correct:
-      "\<And>vaddress acctype iswrite wasaligned size iswritevalidcap addrdesc e.
-          Run (AArch64_FullTranslateWithTag vaddress acctype iswrite wasaligned size iswritevalidcap) t addrdesc \<Longrightarrow>
-          \<forall>e' \<in> set t. translation_assms e' \<Longrightarrow>
-          e \<in> set t \<Longrightarrow> is_mem_event e \<Longrightarrow>
-          is_translation_event e"
-    and no_cap_load_translation_events: "\<And>rk addr sz data. \<not>is_translation_event (E_read_memt rk addr sz data)"
-    and translation_el: "\<And>t acctype el. Run (AArch64_AccessUsesEL acctype) t el \<Longrightarrow> \<forall>e \<in> set t. translation_assms e \<Longrightarrow> translation_el acctype = el"
-    and s1_enabled: "\<And>t acctype s1e. Run (AArch64_IsStageOneEnabled acctype) t s1e \<Longrightarrow> \<forall>e \<in> set t. translation_assms e \<Longrightarrow> s1_enabled acctype = s1e"
-    and tbi_enabled: "\<And>t acctype addr top. Run (AddrTop addr (translation_el acctype)) t top \<Longrightarrow> \<forall>e \<in> set t. translation_assms e \<Longrightarrow> tbi_enabled acctype (unat addr) = (top \<noteq> 63)"
-    and in_host: "\<And>t acctype ih. Run (ELIsInHost (translation_el acctype)) t ih \<Longrightarrow> \<forall>e \<in> set t. translation_assms e \<Longrightarrow> in_host acctype = ih"
-    and translate_address_valid: "\<And>vaddr acctype paddr. translate_address vaddr = Some paddr \<Longrightarrow> valid_address acctype vaddr"
-    and translate_bounds_address: "\<And>vaddr acctype. valid_address acctype vaddr \<Longrightarrow> translate_address (bounds_address acctype vaddr) = translate_address vaddr"
-    (* Memory pages are at least 4KB in AArch64 *)
-    and translate_address_paged: "\<And>vaddr vaddr' paddr. translate_address vaddr = Some paddr \<Longrightarrow> vaddr' div 2^12 = vaddr div 2^12 \<Longrightarrow> translate_address vaddr' = Some (2^12 * (paddr div 2^12) + vaddr' mod 2^12)"
-    (*and translate_address_paged: "\<And>vaddr vaddr' acctype paddr paddr'. translate_address vaddr acctype = Some paddr \<Longrightarrow> translate_address vaddr' acctype = Some paddr' \<Longrightarrow> vaddr div 2^12 = vaddr' div 2^12 \<Longrightarrow> paddr div 2^12 = paddr' div 2^12"
-    and translate_address_page_offset: "\<And>vaddr acctype paddr. translate_address vaddr acctype = Some paddr \<Longrightarrow> paddr mod 2^12 = vaddr mod 2^12"*)
-    and AArch64_TakeException_raises_isa_ex:
-      "exp_raises_isa_ex (AArch64_TakeException target_el exception preferred_exception_return vect_offset)"
-begin
-
-lemma translate_address_page_offset:
-  assumes "translate_address vaddr = Some paddr"
-  shows "paddr mod 2^12 = vaddr mod 2^12"
-proof -
-  have *: "2^12 * (paddr div 2^12) + vaddr mod 2^12 = paddr"
-    using assms translate_address_paged[of vaddr paddr vaddr]
-    by auto
-  have "(2^12 * (paddr div 2^12) + vaddr mod 2^12) mod 2^12 = vaddr mod 2^12"
-    by simp
-  then show ?thesis
-    unfolding *
-    .
-qed
-
-lemma translate_address_aligned_iff[simp]:
-  assumes "translate_address vaddr = Some paddr"
-    and "sz dvd 2^12"
-  shows "aligned paddr sz \<longleftrightarrow> aligned vaddr sz"
-proof -
-  have "aligned paddr sz \<longleftrightarrow> aligned (2^12 * (paddr div 2^12) + vaddr mod 2^12) sz"
-    using assms translate_address_paged[OF assms(1), where vaddr' = vaddr]
-    by auto
-  also have "\<dots> \<longleftrightarrow> aligned vaddr sz"
-    using assms(2)
-    by (auto simp: aligned_def dvd_add_right_iff dvd_mod_iff)
-  finally show ?thesis
-    .
-qed
-
-lemma AArch64_FullTranslate_translate_address[simp]:
-  assumes "Run (AArch64_FullTranslate vaddress acctype iswrite wasaligned sz) t addrdesc"
-    and "\<not>IsFault addrdesc" and "\<forall>e \<in> set t. translation_assms e"
-  shows "translate_address (unat vaddress) = Some (unat (FullAddress_address (AddressDescriptor_paddress addrdesc)))"
-  using assms
-  by (auto simp: AArch64_FullTranslate_def IsFault_def elim!: Run_bindE Run_ifE)
-
-lemma AArch64_TranslateAddressWithTag_translate_address[simp]:
-  assumes "Run (AArch64_TranslateAddressWithTag vaddress acctype iswrite wasaligned sz iswritevalidcap) t addrdesc"
-    and "\<not>IsFault addrdesc" and "\<forall>e \<in> set t. translation_assms e"
-  shows "translate_address (unat vaddress) = Some (unat (FullAddress_address (AddressDescriptor_paddress addrdesc)))"
-  using assms
-  by (auto simp: AArch64_TranslateAddressWithTag_def IsFault_def elim!: Run_bindE Run_ifE)
-
-lemma AArch64_TranslateAddress_translate_address[simp]:
-  assumes "Run (AArch64_TranslateAddress vaddress acctype iswrite wasaligned sz) t addrdesc"
-    and "\<not>IsFault addrdesc" and "\<forall>e \<in> set t. translation_assms e"
-  shows "translate_address (unat vaddress) = Some (unat (FullAddress_address (AddressDescriptor_paddress addrdesc)))"
-  using assms
-  by (auto simp: AArch64_TranslateAddress_def IsFault_def elim!: Run_bindE Run_ifE)
-
-lemma AArch64_TranslateAddressForAtomicAccess_translate_address[simp]:
-  assumes "Run (AArch64_TranslateAddressForAtomicAccess vaddress sz) t addrdesc"
-    and "\<not>IsFault addrdesc" and "\<forall>e \<in> set t. translation_assms e"
-  shows "translate_address (unat vaddress) = Some (unat (FullAddress_address (AddressDescriptor_paddress addrdesc)))"
-  using assms
-  by (auto simp: AArch64_TranslateAddressForAtomicAccess_def IsFault_def elim!: Run_bindE Run_ifE Run_letE)
-
-sublocale Morello_ISA where translate_address = "\<lambda>addr _. translate_address addr"
-  using no_cap_load_translation_events AArch64_TakeException_raises_isa_ex
-  by unfold_locales auto
-
-sublocale Capability_ISA_Fixed_Translation CC ISA UNKNOWN_caps translation_assms
-  by unfold_locales (auto simp: ISA_def)
-
-end
 
 text \<open>Instantiation of @{term translate_address} for version of spec with translation stubs\<close>
 
@@ -2275,7 +2293,7 @@ lemma no_reg_writes_to_CapIsSystemAccessEnabled[no_reg_writes_toI]:
 
 section \<open>Verification framework\<close>
 
-locale Morello_Cap_Axiom_Automaton = Morello_Fixed_Address_Translation + Cap_Axiom_Automaton CC ISA UNKNOWN_caps enabled use_mem_caps
+locale Morello_Cap_Axiom_Automaton = Morello_ISA + Cap_Axiom_Automaton CC ISA UNKNOWN_caps enabled use_mem_caps
   for enabled :: "(Capability, register_value) axiom_state \<Rightarrow> register_value event \<Rightarrow> bool"
     and use_mem_caps :: bool +
   fixes no_system_reg_access :: bool
@@ -5748,7 +5766,7 @@ lemma BranchTaken_or_PCC_accessible:
 
 end
 
-locale Morello_Load_Cap_Assms = Morello_Fixed_Address_Translation +
+locale Morello_Load_Cap_Assms = Morello_ISA +
   fixes enabled :: "(Capability, register_value) axiom_state \<Rightarrow> register_value event \<Rightarrow> bool"
     and load_auth :: "load_auth option" and load_caps_permitted :: "bool"
     and no_system_reg_access :: bool
@@ -6058,7 +6076,7 @@ lemma load_instr_exp_assms_write_ThisInstrAbstract_iff:
 
 end
 
-locale Morello_Cap_Invocation_Assms = Morello_Fixed_Address_Translation +
+locale Morello_Cap_Invocation_Assms = Morello_ISA +
   fixes enabled :: "(Capability, register_value) axiom_state \<Rightarrow> register_value event \<Rightarrow> bool"
     and use_mem_caps :: "bool"
     and instr_opt :: "instr_ast option"
@@ -6605,7 +6623,7 @@ lemmas tagged_mem_primitives_invoked_caps[derivable_capsE] =
 
 end
 
-locale Morello_Axiom_Assms = Morello_Fixed_Address_Translation +
+locale Morello_Axiom_Assms = Morello_ISA +
   fixes enabled :: "(Capability, register_value) axiom_state \<Rightarrow> register_value event \<Rightarrow> bool"
     and ex_traces :: bool
     and instr_opt :: "instr_ast option"
@@ -6656,7 +6674,7 @@ lemma BranchAddr_not_sealed:
   unfolding BranchAddr_def
   by (auto elim!: Run_bindE Run_letE split: if_splits)
 
-lemma branch_caps_128th_iff:
+lemma (in Morello_ISA) branch_caps_128th_iff:
   assumes "c' \<in> branch_caps c"
   shows "c' !! 128 \<longleftrightarrow> c !! 128"
   using assms
@@ -6666,24 +6684,37 @@ lemma leq_cap_CapWithTagClear[simp, intro]:
   "leq_cap CC (CapWithTagClear c) c'"
   by (auto simp: leq_cap_def)
 
-lemma BranchAddr_in_branch_caps:
-  assumes "Run (BranchAddr c el) t c'" and "CapIsTagSet c'"
+lemma (in Morello_ISA) BranchAddr_in_branch_caps:
+  assumes "Run (BranchAddr c el) t c'"
+    and "CapIsTagSet c'"
+    and "translation_el AccType_IFETCH = el"
+    and "translation_assms_trace t"
   shows "c' \<in> branch_caps c"
   using assms
   unfolding BranchAddr_def branch_caps_def
+  thm tbi_enabled
   by (cases "CapIsSealed c")
-     (auto elim!: Run_bindE Run_letE Run_ifE Run_and_boolM_E Run_or_boolM_E
+     (auto elim!: Run_bindE Run_letE Run_ifE Run_and_boolM_E Run_or_boolM_E dest!: tbi_enabled
            simp: CapSetFlags_mask_56_normalise_cursor_flags CapSetFlags_SignExtend_normalise_cursor_flags)
 
-lemma BranchAddr_branch_caps_tagged_unsealed:
+lemma (in Morello_ISA) BranchAddr_branch_caps_tagged_unsealed:
   assumes "Run (BranchAddr c el) t c'" and "CapIsTagSet c'"
+    and "translation_el AccType_IFETCH = el"
+    and "translation_assms_trace t"
   obtains "c' \<in> branch_caps c" and "CapIsTagSet c" and "\<not>CapIsSealed c"
-  sorry
+  using BranchAddr_in_branch_caps[OF assms] assms
+  by (auto simp: BranchAddr_def Let_def elim!: Run_bindE split: if_splits)
 
-lemma branch_caps_set_bit_0_subset:
+lemma bin_nth_int_unat[simp]:
+  "bin_nth (int (unat w)) n = w !! n"
+  unfolding test_bit_def' uint_nat
+  ..
+
+lemma (in Morello_ISA) branch_caps_set_bit_0_subset:
   assumes "\<not>CapIsSealed c"
   shows "branch_caps (set_bit c 0 False) \<subseteq> branch_caps c"
-  by (use assms in \<open>auto simp: branch_caps_def normalise_cursor_flags_def CapGetValue_set_bit_commute test_bit_set_gen\<close>)
+  using assms tbi_enabled_cong[of "unat (CapGetValue c)" "unat (set_bit (CapGetValue c) 0 False)" AccType_IFETCH]
+  by (auto simp: branch_caps_def normalise_cursor_flags_def CapGetValue_set_bit_commute test_bit_set_gen)
 
 locale Morello_Axiom_Automaton =
   Morello_Axiom_Assms +
@@ -6802,7 +6833,7 @@ proof cases
   then show ?thesis
     using assms
     unfolding branch_caps_def normalise_cursor_flags_def
-    by (auto intro: leq_cap_set_0th leq_cap_CapSetFlags leq_cap_CapSetFlags[THEN leq_cap_trans])
+    by (auto intro: leq_cap_set_0th leq_cap_CapSetFlags leq_cap_CapSetFlags[THEN leq_cap_trans] split: if_splits)
 next
   assume "\<not>CapIsTagSet c"
   then have "\<not>CapIsTagSet c'"
@@ -6869,7 +6900,7 @@ lemma not_is_fetchE[elim, derivable_capsE]:
 
 end
 
-locale Morello_Write_Cap_Automaton = Morello_Fixed_Address_Translation +
+locale Morello_Write_Cap_Automaton = Morello_ISA +
   fixes ex_traces :: bool
     and instr_opt :: "instr_ast option"
     and invoked_code_caps :: "Capability set"
@@ -6913,12 +6944,7 @@ locale Morello_Fetch_Write_Cap_Automaton = Morello_Write_Cap_Automaton + Morello
 (* sublocale Morello_Instr_Write_Cap_Automaton \<subseteq> Morello_Instr_Axiom_Automaton where enabled = enabled .. *)
 (* sublocale Morello_Fetch_Write_Cap_Automaton \<subseteq> Morello_Fetch_Axiom_Automaton where enabled = enabled .. *)
 
-(* Assume stubbed out address translation for now *)
-locale Morello_Mem_Axiom_Automaton =
-  Morello_Fixed_Address_Translation
-  (*where translate_address = translate_address
-    and is_translation_event = "\<lambda>_. False"
-    and translation_assms = "\<lambda>_. True"*) +
+locale Morello_Mem_Axiom_Automaton = Morello_ISA +
   fixes ex_traces :: bool
     and instr_opt :: "instr_ast option"
     and invoked_code_caps :: "Capability set"
@@ -6928,12 +6954,6 @@ locale Morello_Mem_Axiom_Automaton =
     and no_system_reg_access :: bool
     and is_in_c64 :: bool
     and is_fetch :: "bool"
-    (*and invoked_caps :: "Capability set" and invoked_regs :: "int set"
-    and invoked_indirect_caps :: "Capability set" and invoked_indirect_regs :: "int set"
-    and load_auths :: "load_auth set" and load_caps_permitted :: "bool" and is_fetch :: "bool"
-    and no_system_reg_access :: bool
-    and is_in_c64 :: bool
-    and is_indirect_branch :: bool*)
 begin
 
 sublocale Mem_Automaton
@@ -6988,7 +7008,7 @@ locale Morello_Fetch_Mem_Automaton = Morello_Mem_Axiom_Automaton + Morello_Fetch
   (* where translate_address = "\<lambda>addr _ _. translate_address addr" and enabled = enabled .. *)
   (* where enabled = enabled .. *)
 
-locale Morello_Trace_Axiom_Automaton = Morello_Fixed_Address_Translation +
+locale Morello_Trace_Axiom_Automaton = Morello_ISA +
   Morello_Axiom_Automaton
   where ex_traces = "isa.trace_raises_ex ISA t"
     and instr_opt = "instr_of_trace (trace t)"
@@ -7002,7 +7022,7 @@ locale Morello_Trace_Axiom_Automaton = Morello_Fixed_Address_Translation +
     and is_fetch = "is_fetch_trace t"
   for t :: "(register_value, instr) isa_trace"
 
-locale Morello_Trace_Write_Cap_Automaton = Morello_Fixed_Address_Translation +
+locale Morello_Trace_Write_Cap_Automaton = Morello_ISA +
   Morello_Write_Cap_Automaton
   where ex_traces = "isa.trace_raises_ex ISA t"
     and instr_opt = "instr_of_trace (trace t)"
@@ -7018,7 +7038,7 @@ locale Morello_Trace_Write_Cap_Automaton = Morello_Fixed_Address_Translation +
 
 sublocale Morello_Trace_Write_Cap_Automaton \<subseteq> Morello_Trace_Axiom_Automaton where t = t and enabled = enabled ..
 
-locale Morello_Trace_Mem_Automaton = Morello_Fixed_Address_Translation +
+locale Morello_Trace_Mem_Automaton = Morello_ISA +
   Morello_Mem_Axiom_Automaton
   where ex_traces = "isa.trace_raises_ex ISA t"
     and instr_opt = "instr_of_trace (trace t)"
